Add support for splitting multiplication
This adds a rewriting pass (disabled by default) which can split apart
multiplications to emit code in a single integer type.

Note that we can emit PHOAS code with only a single integer type, but to
emit C code, we must also allow uint1; see
https://github.com/mit-plv/fiat-crypto/issues/524#issuecomment-529060374
for more details.

We leave it like this because the bedrock2 translation will be coming
from PHOAS.

Note that we must still permit wider integer types during bounds
analysis, because otherwise we'll fail to assign bounds before we even
get to the point of splitting multipliciations.

Note that this rewriting pass is still admitted, so this commit adds a
dependency on an axiom to the overall pass.  (We could create a separate
pipeline if we wanted the code we're extracting to not depend on this
admitted proof.)

The interesting files to look at here are `src/RewriterRules.v`
(defining the rewriting rules) and `src/SlowPrimeSynthesisExamples.v`
giving examples.  The admitted proof is in `src/RewriterRulesProofs.v`.

src/BoundsPipeline.v
@@ -113,6 +113,26 @@ Qed.
 
 Class static_opt := static : bool.
 Typeclasses Opaque static_opt.
+Class split_mul_to_opt := split_mul_to : option (Z * Z).
+Typeclasses Opaque split_mul_to_opt.
+Class should_split_mul_opt := should_split_mul : bool.
+Typeclasses Opaque should_split_mul_opt.
+Class widen_carry_opt := widen_carry : bool.
+Typeclasses Opaque widen_carry_opt.
+Class widen_bytes_opt := widen_bytes : bool.
+Typeclasses Opaque widen_bytes_opt.
+Notation split_mul_to_of_should_split_mul machine_wordsize possible_bitwidths
+  := (if should_split_mul return split_mul_to_opt
+      then Some (machine_wordsize, fold_right Z.min machine_wordsize (filter (fun x => (1 <=? x)%Z) possible_bitwidths))
+      else None) (only parsing).
+(* We include [0], so that even after bounds relaxation, we can
+   notice where the constant 0s are, and remove them. *)
+Notation prefix_with_carry bitwidths :=
+  ((if widen_carry then (0::bitwidths) else (0::1::bitwidths))%Z)
+    (only parsing).
+Notation prefix_with_carry_bytes bitwidths :=
+  (prefix_with_carry (if widen_bytes then bitwidths else 8::bitwidths)%Z)
+    (only parsing).
 
 Module Pipeline.
   Import GeneralizeVar.
@@ -299,6 +319,7 @@ Module Pipeline.
        E.
 
   Definition BoundsPipeline
+             {split_mul_to : split_mul_to_opt}
              (with_dead_code_elimination : bool := true)
              (with_subst01 : bool)
              (translate_to_fancy : option to_fancy_args)
@@ -324,6 +345,11 @@ Module Pipeline.
       match E' with
       | inl E
         => let E := RewriteAndEliminateDeadAndInline RewriteRules.RewriteArithWithCasts with_dead_code_elimination with_subst01 E in
+           let E := match split_mul_to with
+                    | Some (max_bitwidth, lgcarrymax)
+                      => RewriteRules.RewriteMulSplit max_bitwidth lgcarrymax E
+                    | None => E
+                    end in
            let E := match translate_to_fancy with
                     | Some {| invert_low := invert_low ; invert_high := invert_high ; value_range := value_range ; flag_range := flag_range |}
                       => RewriteRules.RewriteToFancyWithCasts invert_low invert_high value_range flag_range E
@@ -340,6 +366,7 @@ Module Pipeline.
   Definition BoundsPipelineToStrings
              {output_language_api : ToString.OutputLanguageAPI}
              {static : static_opt}
+             {split_mul_to : split_mul_to_opt}
              (type_prefix : string)
              (name : string)
              (with_dead_code_elimination : bool := true)
@@ -371,6 +398,7 @@ Module Pipeline.
   Definition BoundsPipelineToString
              {output_language_api : ToString.OutputLanguageAPI}
              {static : static_opt}
+             {split_mul_to : split_mul_to_opt}
              (type_prefix : string)
              (name : string)
              (with_dead_code_elimination : bool := true)
@@ -396,10 +424,10 @@ Module Pipeline.
        end.
 
   Local Notation arg_bounds_of_pipeline result
-    := ((fun a b c t E arg_bounds out_bounds result' (H : @Pipeline.BoundsPipeline a b c t E arg_bounds out_bounds = result') => arg_bounds) _ _ _ _ _ _ _ result eq_refl)
+    := ((fun a b c d t E arg_bounds out_bounds result' (H : @Pipeline.BoundsPipeline a b c d t E arg_bounds out_bounds = result') => arg_bounds) _ _ _ _ _ _ _ _ result eq_refl)
          (only parsing).
   Local Notation out_bounds_of_pipeline result
-    := ((fun a b c t E arg_bounds out_bounds result' (H : @Pipeline.BoundsPipeline a b c t E arg_bounds out_bounds = result') => out_bounds) _ _ _ _ _ _ _ result eq_refl)
+    := ((fun a b c d t E arg_bounds out_bounds result' (H : @Pipeline.BoundsPipeline a b c d t E arg_bounds out_bounds = result') => out_bounds) _ _ _ _ _ _ _ _ result eq_refl)
          (only parsing).
 
   Notation FromPipelineToString prefix name result
@@ -465,6 +493,7 @@ Module Pipeline.
 
   Local Opaque RewriteAndEliminateDeadAndInline.
   Lemma BoundsPipeline_correct
+             {split_mul_to : split_mul_to_opt}
              (with_dead_code_elimination : bool := true)
              (with_subst01 : bool)
              (translate_to_fancy : option to_fancy_args)
@@ -515,7 +544,7 @@ Module Pipeline.
       { subst; split; [ | solve [ wf_interp_t ] ].
         split_and; simpl in *.
         split; [ solve [ wf_interp_t; eauto with nocore ] | ].
-        intros; break_innermost_match; autorewrite with interp; try solve [ wf_interp_t ]; [ | ].
+        intros; break_innermost_match; autorewrite with interp; try solve [ wf_interp_t ].
         all: match goal with H : context[type.app_curried _ _ = _] |- _ => erewrite H; clear H end; eauto.
         all: transitivity (type.app_curried (Interp (PartialEvaluateWithListInfoFromBounds e arg_bounds)) arg1);
           [ | apply Interp_PartialEvaluateWithListInfoFromBounds; auto ].
@@ -541,6 +570,7 @@ Module Pipeline.
        /\ Wf rv.
 
   Lemma BoundsPipeline_correct_trans
+        {split_mul_to : split_mul_to_opt}
         (with_dead_code_elimination : bool := true)
         (with_subst01 : bool)
         (translate_to_fancy : option to_fancy_args)
