src/PushButtonSynthesis/BarrettReduction.v
@@ -55,6 +55,8 @@ Section rbarrett_red.
     := [1; machine_wordsize / 2; machine_wordsize; 2 * machine_wordsize]%Z.
   Let possible_values := possible_values_of_machine_wordsize.
 
+  Local Instance split_mul_to : split_mul_to_opt := None.
+
   Let fancy_args
     := (Some {| Pipeline.invert_low log2wordsize := invert_low log2wordsize consts_list;
                 Pipeline.invert_high log2wordsize := invert_high log2wordsize consts_list;
