src/RewriterAll.v
@@ -2,6 +2,7 @@ Require Import Crypto.Rewriter.NBE.
 Require Import Crypto.Rewriter.Arith.
 Require Import Crypto.Rewriter.ArithWithCasts.
 Require Import Crypto.Rewriter.StripLiteralCasts.
+Require Import Crypto.Rewriter.MulSplit.
 Require Import Crypto.Rewriter.ToFancy.
 Require Import Crypto.Rewriter.ToFancyWithCasts.
 
@@ -10,6 +11,7 @@ Module Compilers.
   Export Arith.Compilers.
   Export ArithWithCasts.Compilers.
   Export StripLiteralCasts.Compilers.
+  Export MulSplit.Compilers.
   Export ToFancy.Compilers.
   Export ToFancyWithCasts.Compilers.
 
@@ -18,6 +20,7 @@ Module Compilers.
     Export Arith.Compilers.RewriteRules.
     Export ArithWithCasts.Compilers.RewriteRules.
     Export StripLiteralCasts.Compilers.RewriteRules.
+    Export MulSplit.Compilers.RewriteRules.
     Export ToFancy.Compilers.RewriteRules.
     Export ToFancyWithCasts.Compilers.RewriteRules.
   End RewriteRules.
